Refactoring & redoing maps

src/AncillaHeap.fst
@@ -1,23 +1,23 @@
-﻿module AncillaHeap
+﻿(** Ancilla heaps with an infinite supply of unique ancillas *)
+module AncillaHeap
 
-(* AncillaHeap - Heaps of integers along with an allocator. The allocator gives
-                 a value greater than every previously allocated value if the
-                 user tries to get the min of an empty heap. Used to implement
-                 bit allocation & retrieval *)
+(* Heaps of integers along with an allocator. The allocator gives
+   a value greater than every previously allocated value if the
+   user tries to get the min of an empty heap. Used to implement
+   bit allocation & retrieval *)
 
-open Util
-open PairHeap
+open Set
 open Total
-
-// (Effectively) infinite sets of address
+open PairHeap
 
 type AncHeapRecord = { hp:intHeap; max:int }
-type cond (ah:AncHeapRecord) = is_heap ah.hp /\ (forall i. (PairHeap.mem i ah.hp ==> i < ah.max))
+type cond (ah:AncHeapRecord) = 
+  is_heap ah.hp /\ (forall i. (PairHeap.mem i ah.hp ==> i < ah.max))
+(* Correctness is encoded in the type *)
 type AncHeap = ah:AncHeapRecord{cond ah}
 
 val emptyHeap : AncHeap
-val above : int -> Tot AncHeap
-
+val above     : int -> Tot AncHeap
 val maxUsed   : AncHeap -> Tot int
 val dat       : AncHeap -> Tot intHeap
 val insert    : AncHeap -> int -> Tot AncHeap
@@ -25,7 +25,6 @@ val popMin    : AncHeap -> Tot (AncHeap * int)
 val getn      : AncHeap -> nat -> Tot (AncHeap * list int)
 val getn_acc  : AncHeap -> (list int) -> n:nat -> Tot (AncHeap * list int) (decreases n)
 val mem       : int -> AncHeap -> Tot bool
-val elts      : AncHeap -> Tot (set int)
 
 let emptyHeap = { hp = Empty; max = 0 }
 let above n   = { hp = Empty; max = n }
@@ -52,22 +51,24 @@ let rec getn_acc ah acc n = match n with
 let getn ah n = getn_acc ah [] n
 
 let mem i ah = if i >= ah.max then true else PairHeap.mem i ah.hp
+
+(** Verification utilities *)
+val elts      : AncHeap -> Tot (set int)
+val get_min    : AncHeap -> Tot int
+val delete_min : AncHeap -> Tot AncHeap
+
+let get_min ah = snd (popMin ah)
+let delete_min ah = fst (popMin ah)
 let elts ah = fun i -> mem i ah
 
-// -------------------------------------------------- Ancilla PairHeap properties
-// Do not use these outside of proofs -- very inefficient
-val get_min    : AncHeap -> Tot int
-let get_min ah = snd (popMin ah)
-val delete_min : AncHeap -> Tot AncHeap
-let delete_min ah = fst (popMin ah)
-
-
-// Zero valued PairHeaps
-type zeroHeap (st:state) (ah:AncHeap) = forall i. (mem i ah) ==> (st i = false)
+(* Ancilla heaps with all zero values *)
+type zeroHeap (st:state) (ah:AncHeap) = 
+  forall i. (mem i ah) ==> (lookup st i = false)
 
 val pop_is_zero : st:state -> ah:AncHeap ->
   Lemma (requires (zeroHeap st ah))
-        (ensures (st (snd (popMin ah)) = false)) [SMTPat (st (snd (popMin ah)))]
+        (ensures (lookup st (snd (popMin ah)) = false)) 
+  [SMTPat (lookup st (snd (popMin ah)))]
 let pop_is_zero st ah = ()
 
 val max_increasing : ah:AncHeap ->
@@ -102,12 +103,12 @@ val zeroHeap_subset : st:state -> ah:AncHeap -> ah':AncHeap ->
 let zeroHeap_subset st ah ah' = ()
 
 val zeroHeap_insert : st:state -> ah:AncHeap -> i:int ->
-  Lemma (requires (zeroHeap st ah /\ st i = false))
+  Lemma (requires (zeroHeap st ah /\ lookup st i = false))
         (ensures  (zeroHeap st (insert ah i)))
 let zeroHeap_insert st ah i = ()
 
 val zeroHeap_insert_list : st:state -> ah:AncHeap -> lst:list int ->
-  Lemma (requires (zeroHeap st ah /\ (forall i. List.mem i lst ==> st i = false)))
+  Lemma (requires (zeroHeap st ah /\ (forall i. List.mem i lst ==> lookup st i = false)))
         (ensures  (zeroHeap st (List.fold_leftT insert ah lst)))
   (decreases lst)
 let rec zeroHeap_insert_list st ah lst = match lst with
