src/Circuit.fst
@@ -1,10 +1,11 @@
-﻿module Circuit
+﻿(** Reversible circuit data type & utilities *)
+module Circuit
 
-(* Circuit - Reversible circuit data structure & utilities. Properties proven
-             mainly involve which bits may be modified by a circuit, and that
-             various methods of uncomputing a computation are correct *)
+(* Reversible circuit data structure & utilities. Properties proven
+   mainly involve which bits may be modified by a circuit, and that
+   various methods of uncomputing a computation are correct *)
 
-open Util
+open Set
 open Total
 
 type Gate =
@@ -12,14 +13,24 @@ type Gate =
   | RTOFF of int * int * int
   | RNOT  of int
 
-type Circuit =
-  { gates : list Gate;
-    inputs : list (string * int);
-    outputs : list int;
-    ancilla : int }
+type Circuit = list Gate
 
-// Printing
-val prettyPrintGate : Gate -> string
+val prettyPrintGate    : Gate -> string
+val prettyPrintCircuit : Circuit -> list string
+
+val applyGate          : state -> Gate -> Tot state
+val evalCirc           : Circuit -> state -> Tot state
+val wfGate             : Gate -> Tot bool
+val wfCirc             : Circuit -> Tot bool
+val used               : int -> Circuit -> Tot bool
+val uses               : Circuit -> Tot (set int)
+val modded             : int -> Circuit -> Tot bool
+val mods               : Circuit -> Tot (set int)
+val ctrl               : int -> Circuit -> Tot bool
+val ctrls              : Circuit -> Tot (set int)
+val uncompute          : Circuit -> int -> Tot Circuit
+
+(* Printing *)
 let prettyPrintGate gate = match gate with
   | RCNOT (a, b) -> String.strcat "tof "
                    (String.strcat (Prims.string_of_int a)
@@ -31,86 +42,69 @@ let prettyPrintGate gate = match gate with
                       (String.strcat " " (Prims.string_of_int c)))))
   | RNOT a -> String.strcat "tof " (Prims.string_of_int a)
 
-val prettyPrintCircuit : list Gate -> list string
 let prettyPrintCircuit = List.map prettyPrintGate
 
-// Evaluation
-val applyGate : state -> Gate -> Tot state
+(* Evaluation *)
 let applyGate st gate = match gate with
-  | RCNOT (a, b)    -> update st b ((st a) <> (st b))
-  | RTOFF (a, b, c) -> update st c ((st c) <> ((st a) && (st b)))
-  | RNOT  a         -> update st a (not (st a))
+  | RCNOT (a, b)    -> update st b ((lookup st a) <> (lookup st b))
+  | RTOFF (a, b, c) -> update st c ((lookup st c) <> ((lookup st a) && (lookup st b)))
+  | RNOT  a         -> update st a (not (lookup st a))
 
-val evalCirc : list Gate -> state -> Tot state
 let rec evalCirc gates st = match gates with
   | [] -> st
   | x::xs -> evalCirc xs (applyGate st x)
 
-// Well formed
-val wfGate : Gate -> Tot bool
+(* Well formed circuits *)
 let wfGate gate = match gate with
   | RCNOT (a, b) -> not (a = b)
   | RTOFF (a, b, c) -> not (a = c) && not (b = c)
   | RNOT a -> true
 
-val wfCirc : list Gate -> Tot bool
 let rec wfCirc circ = match circ with
   | [] -> true
   | x::xs -> wfGate x && wfCirc xs
 
-// Qubits used by a circuit
-val used : int -> list Gate -> Tot bool
+(* Uses, targets, and controls. Uses mods and ctrls are highly inefficient *)
 let rec used i lst = match lst with
   | [] -> false
   | (RCNOT (a, b))::xs    -> a = i || b = i || used i xs
   | (RTOFF (a, b, c))::xs -> a = i || b = i || c = i || used i xs
   | (RNOT a)::xs          -> a = i || used i xs
-
-val uses : list Gate -> Tot (set int)
 let uses lst = fun i -> used i lst
 
-// Qubits modified by a circuit
-val modded : int -> list Gate -> Tot bool
 let rec modded i gates = match gates with
   | [] -> false
   | (RCNOT (_, t))::xs
   | (RTOFF (_, _, t))::xs
   | (RNOT t)::xs -> i = t || modded i xs
-
-val mods : list Gate -> Tot (set int)
 let mods gates = fun i -> modded i gates
 
-// Qubits used as controls
-val ctrl : int -> list Gate -> Tot bool
 let rec ctrl i lst = match lst with
   | [] -> false
   | (RCNOT (a, b))::xs    -> a = i || ctrl i xs
   | (RTOFF (a, b, c))::xs -> a = i || b = i || ctrl i xs
   | (RNOT a)::xs          -> ctrl i xs
-
-val ctrls : list Gate -> Tot (set int)
 let ctrls gates = fun i -> ctrl i gates
 
-// Uncompute relative a target bit
-val uncompute : list Gate -> int -> Tot (list Gate)
+(* Uncompute relative a target bit *)
 let rec uncompute circ targ = match circ with
   | [] -> []
   | x::xs -> if (used targ [x]) then uncompute xs targ else x::(uncompute xs targ)
 
-// ---------------------------------------------------------- Circuit properties
+(** Verification utilities *)
 
-// Lemmas about modified bits
-val ref_imp_use : gates:(list Gate) ->
+(* Lemmas about modified bits *)
+val ref_imp_use : gates:Circuit ->
   Lemma (forall i. modded i gates \/ ctrl i gates <==> used i gates)
 let rec ref_imp_use gates = match gates with
   | [] -> ()
   | x::xs -> ref_imp_use xs
 
-val mods_sub_uses : gates:list Gate ->
+val mods_sub_uses : gates:Circuit ->
   Lemma (subset (mods gates) (uses gates))
 let mods_sub_uses gates = ref_imp_use gates
 
-val ctrls_sub_uses : gates:list Gate ->
+val ctrls_sub_uses : gates:Circuit ->
   Lemma (subset (ctrls gates) (uses gates))
 let ctrls_sub_uses gates = ref_imp_use gates
 
@@ -118,15 +112,15 @@ val apply_mod : st:state -> x:Gate ->
   Lemma (agree_on st (applyGate st x) (complement (mods [x])))
 let apply_mod st x = ()
 
-val eval_mod : st:state -> gates:(list Gate) ->
+val eval_mod : st:state -> gates:Circuit ->
   Lemma (agree_on st (evalCirc gates st) (complement (mods gates)))
 let rec eval_mod st gates = match gates with
   | [] -> ()
   | x::xs -> apply_mod st x; eval_mod (applyGate st x) xs
 
-// Append lemmas, uses SMTPat to expand out automatically (hopefully)
+(* Append lemmas, uses SMTPat to expand out automatically *)
 
-val evalCirc_append : l1:(list Gate) -> l2:(list Gate) -> st:state ->
+val evalCirc_append : l1:Circuit -> l2:Circuit -> st:state ->
   Lemma (requires true)
         (ensures (evalCirc (l1@l2) st = evalCirc l2 (evalCirc l1 st)))
   [SMTPat (evalCirc (l1@l2) st)]
@@ -134,7 +128,7 @@ let rec evalCirc_append l1 l2 st = match l1 with
   | [] -> ()
   | x::xs -> evalCirc_append xs l2 (applyGate st x)
 
-val use_append : i:int -> x:(list Gate) -> y:(list Gate) ->
+val use_append : i:int -> x:Circuit -> y:Circuit ->
   Lemma (requires true)
         (ensures  (used i (x@y) <==> used i x \/ used i y))
   [SMTPat (used i (x@y))]
@@ -142,14 +136,14 @@ let rec use_append i x y = match x with
   | [] -> ()
   | x::xs -> use_append i xs y
 
-val uses_append : x:(list Gate) -> y:(list Gate) ->
+val uses_append : x:Circuit -> y:Circuit ->
   Lemma (requires true)
         (ensures  (uses (x@y) = union (uses x) (uses y)))
   [SMTPat (uses (x@y))]
 let rec uses_append x y =
   lemma_equal_intro (uses (x@y)) (union (uses x) (uses y))
 
-val mod_append : i:int -> l1:(list Gate) -> l2:(list Gate) ->
+val mod_append : i:int -> l1:Circuit -> l2:Circuit ->
   Lemma (requires true)
         (ensures  (modded i (l1@l2) <==> modded i l1 \/ modded i l2))
   [SMTPat (modded i (l1@l2))]
@@ -157,14 +151,14 @@ let rec mod_append i l1 l2 = match l1 with
   | [] -> ()
   | x::xs -> mod_append i xs l2
 
-val mods_append : x:(list Gate) -> y:(list Gate) ->
+val mods_append : x:Circuit -> y:Circuit ->
   Lemma (requires true)
         (ensures  (mods (x@y) = union (mods x) (mods y)))
   [SMTPat (mods (x@y))]
 let rec mods_append x y =
   lemma_equal_intro (mods (x@y)) (union (mods x) (mods y))
 
-val ctrl_append : i:int -> x:(list Gate) -> y:(list Gate) ->
+val ctrl_append : i:int -> x:Circuit -> y:Circuit ->
   Lemma (requires true)
         (ensures  (ctrl i (x@y) <==> ctrl i x \/ ctrl i y))
   [SMTPat (ctrl i (x@y))]
@@ -172,14 +166,14 @@ let rec ctrl_append i x y = match x with
   | [] -> ()
   | x::xs -> ctrl_append i xs y
 
-val ctrls_append : x:(list Gate) -> y:(list Gate) ->
+val ctrls_append : x:Circuit -> y:Circuit ->
   Lemma (requires true)
         (ensures  (ctrls (x@y) = union (ctrls x) (ctrls y)))
   [SMTPat (ctrls (x@y))]
 let rec ctrls_append x y =
   lemma_equal_intro (ctrls (x@y)) (union (ctrls x) (ctrls y))
 
-val wf_append : x:list Gate -> y:list Gate ->
+val wf_append : x:Circuit -> y:Circuit ->
   Lemma (requires (wfCirc x /\ wfCirc y))
         (ensures  (wfCirc (x@y)))
   [SMTPat (wfCirc (x@y))]
@@ -187,8 +181,8 @@ let rec wf_append x y = match x with
   | [] -> ()
   | x::xs -> wf_append xs y
 
-// Lemmas about reversibility
-val rev_uses : circ:list Gate ->
+(* Lemmas about reversibility *)
+val rev_uses : circ:Circuit ->
   Lemma (requires true)
         (ensures (uses circ = uses (List.rev circ)))
   [SMTPat (uses (List.rev circ))]
@@ -199,7 +193,7 @@ let rec rev_uses circ = match circ with
     rev_uses xs;
     lemma_equal_intro (uses circ) (uses (List.rev circ))
 
-val rev_mods : circ:list Gate ->
+val rev_mods : circ:Circuit ->
   Lemma (requires true)
         (ensures (mods circ = mods (List.rev circ)))
   [SMTPat (mods (List.rev circ))]
@@ -210,7 +204,7 @@ let rec rev_mods circ = match circ with
     rev_mods xs;
     lemma_equal_intro (mods circ) (mods (List.rev circ))
 
-val rev_ctrls : circ:list Gate ->
+val rev_ctrls : circ:Circuit ->
   Lemma (requires true)
         (ensures (ctrls circ = ctrls (List.rev circ)))
   [SMTPat (ctrls (List.rev circ))]
@@ -221,7 +215,7 @@ let rec rev_ctrls circ = match circ with
     rev_ctrls xs;
     lemma_equal_intro (ctrls circ) (ctrls (List.rev circ))
 
-val evalCirc_append_rev : x:list Gate -> y:list Gate -> st:state ->
+val evalCirc_append_rev : x:Circuit -> y:Circuit -> st:state ->
   Lemma (evalCirc (List.rev (x@y)) st = evalCirc (List.rev x) (evalCirc (List.rev y) st))
 let evalCirc_append_rev x y st = ListProperties.rev_append x y
 
@@ -230,7 +224,7 @@ val rev_gate : gate:Gate -> st:state ->
         (ensures  (applyGate (applyGate st gate) gate = st))
 let rev_gate gate st = lemma_map_equal_intro (applyGate (applyGate st gate) gate) st
 
-val rev_inverse : circ:list Gate -> st:state ->
+val rev_inverse : circ:Circuit -> st:state ->
   Lemma (requires (wfCirc circ))
         (ensures  (evalCirc (circ@(List.rev circ)) st = st))
 let rec rev_inverse circ st = match circ with
@@ -245,7 +239,7 @@ val applyGate_state_swap : x:Gate -> st:state -> st':state -> dom:set int ->
         (ensures  (agree_on (applyGate st x) (applyGate st' x) dom))
 let applyGate_state_swap x st st' dom = ()
 
-val evalCirc_state_swap : circ:list Gate -> st:state -> st':state -> dom:set int ->
+val evalCirc_state_swap : circ:Circuit -> st:state -> st':state -> dom:set int ->
   Lemma (requires (subset (ctrls circ) dom /\ agree_on st st' dom))
         (ensures  (agree_on (evalCirc circ st) (evalCirc circ st') dom))
 let rec evalCirc_state_swap circ st st' dom = match circ with
@@ -254,8 +248,8 @@ let rec evalCirc_state_swap circ st st' dom = match circ with
     applyGate_state_swap x st st' dom;
     evalCirc_state_swap xs (applyGate st x) (applyGate st' x) dom
 
-// Lemmas for uncomputing after copying to a target
-val bennett : comp:list Gate -> copy:list Gate -> st:state ->
+(* Lemmas for uncomputing after copying to a target *)
+val bennett : comp:Circuit -> copy:Circuit -> st:state ->
   Lemma (requires (wfCirc comp /\ disjoint (uses comp) (mods copy)))
         (ensures  (agree_on st (evalCirc (comp@copy@(List.rev comp)) st) (uses comp)))
 let bennett comp copy st =
@@ -266,13 +260,13 @@ let bennett comp copy st =
     evalCirc_state_swap (List.rev comp) st' st'' (uses comp);
     rev_inverse comp st
 
-val uncompute_targ : circ:list Gate -> targ:int ->
+val uncompute_targ : circ:Circuit -> targ:int ->
   Lemma (not (modded targ (uncompute circ targ)))
 let rec uncompute_targ circ targ = match circ with
   | [] -> ()
   | x::xs -> uncompute_targ xs targ
 
-val uncompute_wf : circ:list Gate -> targ:int ->
+val uncompute_wf : circ:Circuit -> targ:int ->
   Lemma (requires (wfCirc circ))
         (ensures  (wfCirc (uncompute circ targ)))
   [SMTPat (wfCirc (uncompute circ targ))]
@@ -280,21 +274,21 @@ let rec uncompute_wf circ targ = match circ with
   | [] -> ()
   | x::xs -> uncompute_wf xs targ
 
-val uncompute_uses_subset : circ:list Gate -> targ:int ->
+val uncompute_uses_subset : circ:Circuit -> targ:int ->
   Lemma (requires (wfCirc circ))
         (ensures  (subset (uses (uncompute circ targ)) (uses circ)))
 let rec uncompute_uses_subset circ targ = match circ with
   | [] -> ()
   | x::xs -> uncompute_uses_subset xs targ
 
-val uncompute_ctrls_subset : circ:list Gate -> targ:int ->
+val uncompute_ctrls_subset : circ:Circuit -> targ:int ->
   Lemma (requires (wfCirc circ))
         (ensures  (subset (ctrls (uncompute circ targ)) (ctrls circ)))
 let rec uncompute_ctrls_subset circ targ = match circ with
   | [] -> ()
   | x::xs -> uncompute_ctrls_subset xs targ
 
-val uncompute_agree : circ:list Gate -> targ:int -> st:state ->
+val uncompute_agree : circ:Circuit -> targ:int -> st:state ->
   Lemma (requires (wfCirc circ /\ not (ctrl targ circ)))
         (ensures  (agree_on (evalCirc circ st)
                             (evalCirc (uncompute circ targ) st)
@@ -313,7 +307,7 @@ let rec uncompute_agree circ targ st = match circ with
     else uncompute_agree xs targ (applyGate st x)
 
 
-val uncompute_mixed_inverse : circ:list Gate -> targ:int -> st:state ->
+val uncompute_mixed_inverse : circ:Circuit -> targ:int -> st:state ->
   Lemma (requires (wfCirc circ /\ not (ctrl targ circ)))
         (ensures  (agree_on st (evalCirc (List.rev (uncompute circ targ))
                                          (evalCirc circ st))
