src/Partial.fst
@@ -1,15 +1,46 @@
-// Partial maps, implemented functionally
+(** Partial maps, implemented as assoc lists *)
 module Partial
-open Util
+open Set
 
-type map (#a:Type) (d:set a) (b:Type) = v:a{d v} -> Tot b
+type t (key:Type) (value:Type) = list (key * value)
 
-val update : #a:Type -> #d:set a -> #b:Type ->
-  map d b -> v:a -> b -> Tot (map (ins v d) b)
-let update d map x y = fun z -> if z = x then y else map z
+val dom      : #key:Type -> #value:Type -> t key value -> Tot (set key)
+val cod      : #key:Type -> #value:Type -> t key value -> Tot (set value)
+val defined  : #key:Type -> #value:Type -> t key value -> key -> Tot bool
+//val empty    : #key:Type -> #value:Type -> Tot (t key value)
+val find     : #key:Type -> #value:Type -> t key value -> key -> Tot (option value)
+val find_def : #key:Type -> #value:Type -> t key value -> key -> value -> Tot value
+val update   : #key:Type -> #value:Type -> t key value -> key -> value -> Tot (t key value)
+val totalize : #key:Type -> #value:Type -> t key value -> value -> Tot (Total.t key value)
 
-val lookup : #a:Type -> d:set a -> #b:Type -> map d b -> x:a{mem x d} -> Tot b
-let lookup d map x = map x
+let rec dom m = match m with
+  | []    -> fun _ -> false
+  | x::xs -> fun y -> (fst x) = y || dom xs y
 
-val dom : #a:Type -> d:set a -> #b:Type -> map d b -> Tot (set a)
-let dom d m = d
+let rec cod m = match m with
+  | []    -> fun _ -> false
+  | x::xs -> fun y -> (snd x) = y || cod xs y
+
+let defined m k = mem k (dom m)
+
+//let empty = []
+
+let rec find m k = List.assocT k m
+
+let rec find_def m k dval = match find m k with
+  | None -> dval 
+  | Some v -> v
+
+let rec update m k v = match m with
+    | [] -> [(k, v)]
+    | (k', v')::xs -> if k = k' then (k, v)::xs else (k', v')::(update xs k v)
+
+let totalize m dval =
+  { Total.elts = m;
+    Total.dval = dval }
+
+(** Verification utilities *)
+val lookup   : #key:Type -> #value:Type -> m:t key value -> k:key{defined m k} -> Tot value
+
+let rec lookup m k = match m with
+  | (k', v)::xs -> if k = k' then v else lookup xs k
