src/Total.fst
@@ -1,53 +1,89 @@
-// Total maps, implemented functionally
+(** Total maps, implemented as assoc lists with default values *)
 module Total
-open Util
+open Set
+
+type t (key:Type) (value:Type) = 
+  { elts : list (key * value);
+    dval : value }
+
+(* type synonym for Boolean-valued states *)
+type state = t int bool
+
+val lookup   : #key:Type -> #value:Type -> t key value -> key -> Tot value
+val update   : #key:Type -> #value:Type -> t key value -> key -> value -> Tot (t key value)
+val constMap : #key:Type -> #value:Type -> value -> Tot (t key value)
+val compose  : #key:Type -> #value:Type -> #value':Type -> t key value -> t value value' -> Tot (t key value')
+val mapVals  : #key:Type -> #value:Type -> #value':Type -> (value -> Tot value') -> t key value -> Tot (t key value')
+
+let lookup m k = match List.assocT k m.elts with
+  | None   -> m.dval
+  | Some v -> v
+
+let update m k v =
+  { elts = (k, v)::m.elts; //(k, v)::(List.filterT (fun (k', _) -> not (k = k')) m.elts);
+    dval = m.dval }
+
+let constMap v =
+  { elts = [];
+    dval = v }
+
+let compose m m' = 
+  { elts = List.mapT (fun (k, v) -> (k, lookup m' v)) m.elts;
+    dval = lookup m' m.dval }
+
+let mapVals f m = 
+  { elts = List.mapT (fun (k, v) -> (k, f v)) m.elts;
+    dval = f m.dval }
+
+
+(** Verification utilities *)
+
+(* Basic equations *)
+val lookup_const : #key:Type -> #value:Type -> k:key -> v:value -> 
+  Lemma (requires true) 
+        (ensures (lookup (constMap v) k = v))
+  [SMTPat (lookup (constMap v) k)]
+val lookup_update1 : #key:Type -> #value:Type -> m:t key value -> k:key -> v:value ->
+  Lemma (requires true)
+        (ensures (lookup (update m k v) k = v))
+  [SMTPat (lookup (update m k v) k)]
+val lookup_update2 : #key:Type -> #value:Type -> m:t key value -> k:key -> v:value -> k':key ->
+  Lemma (requires (not (k = k')))
+        (ensures (lookup (update m k v) k' = lookup m k'))
+  [SMTPat (lookup (update m k v) k')]
+
+let lookup_const k v = ()
+let lookup_update1 m k v = ()
+let lookup_update2 m k v k' = ()
+
+(* Type of maps that agree on a subset of keys *)
+type agree_on (#key:Type) (#value:Type) (m:t key value) (m':t key value) (s:set key) =
+  forall x. mem x s ==> lookup m x = lookup m' x
+
+val agree_on_trans : #key:Type -> #value:Type -> m:t key value -> m':t key value -> m'':t key value -> s:set key ->
+  Lemma (requires (agree_on m m' s /\ agree_on m' m'' s))
+        (ensures  (agree_on m m'' s))
+let agree_on_trans m m' m'' s = ()
+
+
+(* Functional extensionality for lookups *)
 open FStar.FunctionalExtensionality
 
-type map (a:Type) (b:Type) = a -> Tot b
-
-type Equal (#a:Type) (#b:Type) (m1:map a b) (m2:map a b) = FEq m1 m2
-val lemma_map_equal_intro: #a:Type -> #b:Type -> m1:map a b -> m2:map a b ->
-  Lemma (requires  (forall x. m1 x = m2 x))
+type Equal (#key:Type) (#value:Type) (m1:t key value) (m2:t key value) = FEq (lookup m1) (lookup m2)
+val lemma_map_equal_intro: #key:Type -> #value:Type -> m1:t key value -> m2:t key value ->
+  Lemma (requires  (forall x. lookup m1 x = lookup m2 x))
         (ensures   (Equal m1 m2))
   [SMTPatT (Equal m1 m2)]
-val lemma_map_equal_elim: #a:Type -> #b:Type -> m1:map a b -> m2:map a b ->
+val lemma_map_equal_elim: #key:Type -> #value:Type -> m1:t key value -> m2:t key value ->
   Lemma (requires (Equal m1 m2))
-        (ensures  (m1 = m2))
+        (ensures  (lookup m1 = lookup m2))
   [SMTPatT (Equal m1 m2)]
-val lemma_map_equal_refl: #a:Type -> #b:Type -> m1:map a b -> m2:map a b ->
-  Lemma (requires (m1 = m2))
+val lemma_map_equal_refl: #key:Type -> #value:Type -> m1:t key value -> m2:t key value ->
+  Lemma (requires (lookup m1 = lookup m2))
         (ensures  (Equal m1 m2))
   [SMTPatT (Equal m1 m2)]
+
 let lemma_map_equal_intro m1 m2 = ()
 let lemma_map_equal_elim m1 m2 = ()
 let lemma_map_equal_refl m1 m2 = ()
 
-val lookup : #a:Type -> #b:Type -> map a b -> a -> Tot b
-let lookup map x = map x
-
-val lemma_lookup_inline : #a:Type -> #b:Type -> m:map a b -> i:a -> 
-  Lemma (requires true) (ensures (lookup m i = m i))
-  [SMTPat (lookup m i)]
-let lemma_lookup_inline m i = ()
-
-val update : #a:Type -> #b:Type -> map a b -> a -> b -> Tot (map a b)
-let update map x y = fun z -> if z = x then y else map z
-
-val compose : #a:Type -> #b:Type -> #c:Type -> map a b -> map b c -> Tot (map a c)
-let compose m m' = fun i -> m' (m i)
-
-val const_map : #a:Type -> #b:Type -> b -> Tot (map a b)
-let const_map v = fun _ -> v
-
-type state = map int bool
-
-type agree_on (#a:Type) (#b:Type) (mp:map a b) (mp':map a b) (s:set a) =
-  forall x. mem x s ==> mp x = mp' x
-
-val agree_on_trans : #a:Type -> #b:Type -> mp:map a b -> mp':map a b -> mp'':map a b -> s:set a ->
-  Lemma (requires (agree_on mp mp' s /\ agree_on mp' mp'' s))
-        (ensures  (agree_on mp mp'' s))
-let agree_on_trans mp mp' mp'' s = ()
-
-val map_mp : #a:Type -> #b:Type -> (b -> Tot b) -> map a b -> Tot (map a b)
-let map_mp f m = m
