src/Util.fst
@@ -1,88 +1,22 @@
+(** General utilities *)
 module Util
-
-(* Util - General utilities. Sets & set lemmas, monads, list functions *)
+open Set
 
 type fin (n:nat) = m:nat{m <= n}
 
-// Functional sets, strictly for proofs. Mostly identical to Set.fst but
-//   it compiles, hides some definitions, and defines subsets propositionally
-//   rather than computationally
-type set (a:Type) = a -> Tot bool
-
-val mem          : #a:Type -> a -> set a -> Tot bool
-val empty        : #a:Type -> Tot (set a)
-val singleton    : #a:Type -> a -> Tot (set a)
-val union        : #a:Type -> set a -> set a -> Tot (set a)
-val intersection : #a:Type -> set a -> set a -> Tot (set a)
-val complement   : #a:Type -> set a -> Tot (set a)
-val ins          : #a:Type -> a -> set a -> Tot (set a)
-
-let mem i s          = s i
-let empty            = fun _ -> false
-let singleton a      = fun b -> b = a
-let union a b        = fun c -> a c || b c
-let intersection a b = fun c -> a c && b c
-let complement s     = fun x -> not (s x)
-let ins a b          = union (singleton a) b
-
-open FStar.FunctionalExtensionality
-type Equal (#a:Type) (s1:set a) (s2:set a) = FEq s1 s2
-val lemma_equal_intro: #a:Type -> s1:set a -> s2:set a -> Lemma
-    (requires  (forall x. mem x s1 = mem x s2))
-    (ensures (Equal s1 s2))
-    [SMTPatT (Equal s1 s2)]
-val lemma_equal_elim: #a:Type -> s1:set a -> s2:set a -> Lemma
-    (requires (Equal s1 s2))
-    (ensures  (s1 = s2))
-    [SMTPatT (Equal s1 s2)]
-val lemma_equal_refl: #a:Type -> s1:set a -> s2:set a -> Lemma
-    (requires (s1 = s2))
-    (ensures  (Equal s1 s2))
-    [SMTPatT (Equal s1 s2)]
-let lemma_equal_intro s1 s2 = ()
-let lemma_equal_elim s1 s2 = ()
-let lemma_equal_refl s1 s2 = ()
-
-type subset (#a:Type) (s:set a) (s':set a) =
-  forall i. s i ==> s' i
-type disjoint (#a:Type) (s:set a) (s':set a) =
-  forall i. ~(s i /\ s' i)
-
-val subset_trans : #a:Type -> s:set a -> s':set a -> s'':set a ->
-  Lemma (requires (subset s s' /\ subset s' s''))
-        (ensures  (subset s s''))
-let subset_trans s s' s'' = ()
-
-val subset_ins : #a:Type -> i:a -> s:set a ->
-  Lemma (subset s (ins i s))
-let subset_ins i s = ()
-
-val ins_subset_pres : #a:Type -> i:a -> s:set a -> s':set a ->
-  Lemma (requires (subset s s'))
-        (ensures  (subset (ins i s) (ins i s')))
-let ins_subset_pres i s s' = ()
-
-val disjoint_subset : #a:Type -> s:set a -> s':set a -> s'':set a ->
-  Lemma (requires (subset s s' /\ disjoint s' s''))
-        (ensures  (disjoint s s''))
-let disjoint_subset s s' s'' = ()
-
-val disjoint_union : #a:Type -> s:set a -> s':set a -> s'':set a ->
-  Lemma (requires (disjoint s s' /\ disjoint s s''))
-        (ensures  (disjoint s (union s' s'')))
-let disjoint_union s s' s'' = ()
-
-// Error reporting monads
+(** Error reporting monads *)
 type result 'a =
   | Val : 'a -> result 'a
   | Err : string -> result 'a
 
-val get_Val : r:(result 'a){is_Val r} -> Tot 'a
-let get_Val r = match r with
+val getVal : r:(result 'a){is_Val r} -> Tot 'a
+val bind   : result 'a -> ('a -> result 'b) -> result 'b
+val bindT  : result 'a -> ('a -> Tot (result 'b)) -> Tot (result 'b)
+val foldM  : ('a -> 'b -> result 'a) -> 'a -> l:(list 'b) -> result 'a
+
+let getVal r = match r with
   | Val v -> v
 
-val bind : result 'a -> ('a -> result 'b) -> result 'b
-val bindT : result 'a -> ('a -> Tot (result 'b)) -> Tot (result 'b)
 let bind v f = match v with
   | Val x -> f x
   | Err s -> Err s
@@ -90,54 +24,61 @@ let bindT v f = match v with
   | Val x -> f x
   | Err s -> Err s
 
-val foldM : ('a -> 'b -> result 'a) -> 'a -> l:(list 'b) -> result 'a
 let rec foldM f a lst = match lst with
   | [] -> Val a
   | x::xs -> bind (f a x) (fun res -> foldM f res xs)
 
-// Extra list operations
-val mems : #a:Type -> list a -> Tot (set a)
+(** Auxiliary list operations *)
+val mems      : #a:Type -> list a -> Tot (set a)
+val nthT      : l:list 'a -> i:int{i >= 0 && i < List.lengthT l} -> Tot 'a
+val forSomeT  : ('a -> Tot bool) -> list 'a -> Tot bool
+val take      : l:list 'a -> i:int{i <= List.length l} -> Tot (list 'a) (decreases i)
+val remove    : l:list 'a -> i:nat{i < List.length l} -> Tot (list 'a) (decreases i)
+val rotateRec : acc:list 'a -> l:list 'a -> i:nat{i < List.length l} -> Tot (list 'a) (decreases i)
+val rotate    : l:list 'a -> i:nat{i < List.length l} -> Tot (list 'a) (decreases i)
+val slice     : l:list 'a -> i:nat -> j:nat{i <= j && j < List.length l} -> Tot (list 'a)
+val ofInt     : i:nat -> j:int -> Tot (list bool) (decreases j)
+
 let mems l = fun i -> List.mem i l
 
-val nthT : l:list 'a -> i:int{i >= 0 && i < List.lengthT l} -> Tot 'a
 let rec nthT l i = match l with
   | x::xs -> if i = 0 then x else nthT xs (i-1)
 
-val for_someT: ('a -> Tot bool) -> list 'a -> Tot bool
-let rec for_someT f l = match l with
+let rec forSomeT f l = match l with
     | [] -> false
-    | hd::tl -> if f hd then true else for_someT f tl
+    | hd::tl -> if f hd then true else forSomeT f tl
 
-val take : l:(list 'a) -> i:int{i <= List.length l} -> Tot (list 'a) (decreases i)
 let rec take l i =
   if i <= 0 then []
   else match l with
     | x::xs -> x::(take xs (i - 1))
 
-val remove : l:(list 'a) -> i:nat{i < List.length l} ->
-  Tot (l':(list 'a){List.length l' = List.length l - i}) (decreases i)
 let rec remove l i =
   if i = 0 then l
   else match l with
     | _::xs -> remove xs (i - 1)
 
-val rotate_rec : acc:(list 'a) -> l:(list 'a) -> i:nat{i < List.length l} -> Tot (list 'a) (decreases i)
-let rec rotate_rec acc l i =
+(* Need this here so slice will type check *)
+val length_remove : l:list 'a -> i:nat{i < List.length l} -> 
+  Lemma (requires true)
+        (ensures  (List.length (remove l i) = List.length l - i))
+  [SMTPat (List.length (remove l i))]
+let rec length_remove l i = 
+  if i = 0 then ()
+  else match l with
+    | _::xs -> length_remove xs (i - 1)
+
+let rec rotateRec acc l i =
   if i = 0 then acc@(List.rev l)
   else match l with
-    | x::xs -> rotate_rec (x::acc) xs (i-1)
+    | x::xs -> rotateRec (x::acc) xs (i-1)
 
-// Rotates a list by i indices
-val rotate : l:(list 'a) -> i:nat{i < List.length l} -> Tot (list 'a) (decreases i)
 let rotate l i =
   ListProperties.rev_length l;
-  rotate_rec [] (List.rev l) i
+  rotateRec [] (List.rev l) i
 
-val slice : l:(list 'a) -> i:nat -> j:nat{i <= j && j < List.length l} -> Tot (list 'a)
 let slice l i j = take (remove l i) (j - i + 1)
 
-// Generates a list of j Booleans representing the number i mod 2^j
-val of_int : i:nat -> j:int -> Tot (list bool) (decreases j)
-let rec of_int i j =
+let rec ofInt i j =
   if j <= 0 then []
-  else (i % 2 = 1)::(of_int (i / 2) (j - 1))
+  else (i % 2 = 1)::(ofInt (i / 2) (j - 1))
