src/Set.fst
@@ -1,0 +1,74 @@
+(** Functional sets *)
+module Set
+
+(* Strictly for proofs. Mostly identical to Set.fst but
+   it compiles, hides some definitions, and defines subsets propositionally
+   rather than computationally *)
+type set (a:Type) = a -> Tot bool
+
+val mem          : #a:Type -> a -> set a -> Tot bool
+val empty        : #a:Type -> Tot (set a)
+val singleton    : #a:Type -> a -> Tot (set a)
+val union        : #a:Type -> set a -> set a -> Tot (set a)
+val intersection : #a:Type -> set a -> set a -> Tot (set a)
+val complement   : #a:Type -> set a -> Tot (set a)
+val ins          : #a:Type -> a -> set a -> Tot (set a)
+
+let mem i s          = s i
+let empty            = fun _ -> false
+let singleton a      = fun b -> b = a
+let union a b        = fun c -> a c || b c
+let intersection a b = fun c -> a c && b c
+let complement s     = fun x -> not (s x)
+let ins a b          = union (singleton a) b
+
+(** Verification utilities *)
+
+(* Extensionality-based equaltiy *)
+open FStar.FunctionalExtensionality
+type Equal (#a:Type) (s1:set a) (s2:set a) = FEq s1 s2
+val lemma_equal_intro: #a:Type -> s1:set a -> s2:set a -> Lemma
+    (requires  (forall x. mem x s1 = mem x s2))
+    (ensures (Equal s1 s2))
+    [SMTPatT (Equal s1 s2)]
+val lemma_equal_elim: #a:Type -> s1:set a -> s2:set a -> Lemma
+    (requires (Equal s1 s2))
+    (ensures  (s1 = s2))
+    [SMTPatT (Equal s1 s2)]
+val lemma_equal_refl: #a:Type -> s1:set a -> s2:set a -> Lemma
+    (requires (s1 = s2))
+    (ensures  (Equal s1 s2))
+    [SMTPatT (Equal s1 s2)]
+let lemma_equal_intro s1 s2 = ()
+let lemma_equal_elim s1 s2 = ()
+let lemma_equal_refl s1 s2 = ()
+
+(* Subset relation & lemmas *)
+type subset (#a:Type) (s:set a) (s':set a) =
+  forall i. s i ==> s' i
+type disjoint (#a:Type) (s:set a) (s':set a) =
+  forall i. ~(s i /\ s' i)
+
+val subset_trans : #a:Type -> s:set a -> s':set a -> s'':set a ->
+  Lemma (requires (subset s s' /\ subset s' s''))
+        (ensures  (subset s s''))
+let subset_trans s s' s'' = ()
+
+val subset_ins : #a:Type -> i:a -> s:set a ->
+  Lemma (subset s (ins i s))
+let subset_ins i s = ()
+
+val ins_subset_pres : #a:Type -> i:a -> s:set a -> s':set a ->
+  Lemma (requires (subset s s'))
+        (ensures  (subset (ins i s) (ins i s')))
+let ins_subset_pres i s s' = ()
+
+val disjoint_subset : #a:Type -> s:set a -> s':set a -> s'':set a ->
+  Lemma (requires (subset s s' /\ disjoint s' s''))
+        (ensures  (disjoint s s''))
+let disjoint_subset s s' s'' = ()
+
+val disjoint_union : #a:Type -> s:set a -> s':set a -> s'':set a ->
+  Lemma (requires (disjoint s s' /\ disjoint s s''))
+        (ensures  (disjoint s (union s' s'')))
+let disjoint_union s s' s'' = ()
